Verify sequential correctness of the Stencil kernel

Examples/Stencil.v
@@ -2,38 +2,378 @@ Require Import GPUCSL.
 Require Import scan_lib.
 Require Import LibTactics Psatz.
 
-Section Stencil.
-Local Notation smem := (Var "smem").
-Local Notation arr := (Var "arr").
-Local Notation out := (Var "out").
-Local Notation t0 := (Var "t0").
-Local Notation t1 := (Var "t1").
-Local Notation t2 := (Var "t2").
-Local Notation tid := (Var "tid").
-Local Notation bid := (Var "bid").
+Section Stencil_seq.
+Coercion Var : string >-> var.
+(* Local Notation smem := (Var "smem"). *)
+(* Local Notation arr := (Var "arr"). *)
+(* Local Notation out := (Var "out"). *)
+(* Local Notation t0 := (Var "t0"). *)
+(* Local Notation t1 := (Var "t1"). *)
+(* Local Notation t2 := (Var "t2"). *)
+(* Local Notation tid := (Var "tid"). *)
+(* Local Notation bid := (Var "bid"). *)
 
 Variable ntrd nblk : nat.
 Hypothesis ntrd_neq_0 : ntrd <> 0.
 Hypothesis nblk_neq_0 : nblk <> 0.
-
-Local Notation gid := (tid +C bid *C Zn ntrd).
+Open Scope string_scope.
+Local Notation gid := ("tid" +C "bid" *C Zn ntrd).
 
 Definition stencil :=
-  t0 ::= [Gl arr +o gid] ;;
-  [Sh smem +o (tid +C 1%Z)] ::= t0 ;;
-  Cif (tid == 0%Z) (
-    Cif (bid == 0%Z) ([Sh smem +o 0%Z] ::= 0%Z)
-    ( t0 ::= [Gl arr +o (gid -C 1%Z)];; [Sh smem +o 0%Z] ::= t0)
+  "t0" ::= [Gl "arr" +o gid] ;;
+  [Sh "smem" +o ("tid" +C 1%Z)] ::= "t0" ;;
+  Cif ("tid" == 0%Z) (
+    Cif ("bid" == 0%Z) ([Sh "smem" +o 0%Z] ::= 0%Z)
+    ( "t0" ::= [Gl "arr" +o (gid -C 1%Z)];; [Sh "smem" +o 0%Z] ::= "t0" )
   ) (Cskip
   ) ;;
-  Cif (tid == Zn nblk -C 1%Z) (
-    Cif (bid == 0%Z) ([Sh smem +o (Zn ntrd +C 1%Z)] ::= 0%Z)
-    ( t0 ::= [Gl arr +o (gid +C 1%Z)];; [Sh smem +o (Zn ntrd +C 1%Z)] ::= t0)
+  Cif ("tid" == Zn ntrd -C 1%Z) (
+    Cif ("bid" == Zn nblk -C 1%Z) ([Sh "smem" +o (Zn ntrd +C 1%Z)] ::= 0%Z)
+    ( "t0" ::= [Gl "arr" +o (gid +C 1%Z)];; [Sh "smem" +o (Zn ntrd +C 1%Z)] ::= "t0" )
   ) (Cskip
   ) ;;
   Cbarrier 0 ;;
-  t0 ::= [Sh smem +o tid] ;;
-  t1 ::= [Sh smem +o (tid +C 1%Z)] ;;
-  t2 ::= [Sh smem +o (tid +C 2%Z)] ;;
-  [Gl out +o gid] ::= t0 +C t1 +C t2.
+  "t0" ::= [Sh "smem" +o "tid"] ;;
+  "t1" ::= [Sh "smem" +o ("tid" +C 1%Z)] ;;
+  "t2" ::= [Sh "smem" +o ("tid" +C 2%Z)] ;;
+  [Gl "out" +o gid] ::= "t0" +C "t1" +C "t2".
 
+Variable aloc : Z.
+Variable sloc : Z.
+Variable oloc : Z.
+Local Notation nt_gr := (nblk * ntrd).
+Notation perm_n n := (1 / injZ (Zn n))%Qc.
+Variable f : nat -> Z.
+Variable f_sm : nat -> Z.
+Variable f_out : nat -> Z.
+
+Definition f' k := if Sumbool.sumbool_or _ _ _ _ (le_dec k 0) (lt_dec nt_gr k) then 0%Z else f (k - 1).
+
+Notation gi i j := (nf i + nf j * ntrd).
+
+Definition BS0 (j : Fin.t nblk)  : (Vector.t assn ntrd * Vector.t assn ntrd) := 
+  (MyVector.init (fun i =>
+    (Sh sloc +o Zn (nf i + 1) -->p (1, f' (gi i j + 1))) **
+    (if Nat.eq_dec (nf i) 0 then Sh sloc -->p (1, f' ((nf j) * ntrd)) else emp) **
+    (if Nat.eq_dec (nf i) (ntrd - 1) then Sh sloc +o Zn (ntrd + 1) -->p (1, f' ((nf j + 1) * ntrd + 1)) else emp)),
+   MyVector.init (fun i =>
+    is_array_p (Sh sloc) (ntrd + 2) (fun k => f' (k + nf j * ntrd)) 0 (perm_n ntrd))).
+
+Definition BS (j : Fin.t nblk) (n : nat) :=
+  if Nat.eq_dec n 0 then BS0 j else default ntrd.
+
+Lemma stencil_ok_th (j : Fin.t nblk) (i : Fin.t ntrd) :
+  CSL (BS j) i 
+    (!("tid" === Zn (nf i)) **
+     !("bid" === Zn (nf j)) **
+     !("arr" === aloc) **
+     !("out" === oloc) **
+     !("smem" === sloc ) **
+     is_array_p (Gl aloc) nt_gr f 0 (perm_n nt_gr) **
+     (Gl oloc +o Zn (nf i + nf j * ntrd) -->p (1, f_out (nf i + nf j * ntrd))) **
+     (Sh sloc +o Zn (nf i + 1) -->p (1, f_sm (nf i + 1))) **
+     (if Nat.eq_dec (nf i) 0 then Sh sloc -->p (1, f_sm 0) else emp) **
+     (if Nat.eq_dec (nf i) (ntrd - 1) then Sh sloc +o Zn (ntrd + 1) -->p (1, f_sm (ntrd + 1)) else emp))
+    stencil 
+    (is_array_p (Gl aloc) nt_gr f 0 (perm_n nt_gr) **
+     (Gl oloc +o Zn (gi i j) -->p (1, (f' (gi i j) + f' (gi i j + 1) + f' (gi i j + 2)))%Z) **
+     is_array_p (Sh sloc) (ntrd + 2) (fun k => f' (k + nf j * ntrd)) 0 (perm_n ntrd)).
+Proof.
+  assert (Hgi_nt: gi i j < nt_gr) by eauto.
+  unfold stencil.
+  eapply Hbackward.
+  Focus 2. {
+    intros s h H.
+    sep_rewrite_in (@is_array_unfold (Gl aloc) (gi i j)) H; [|eauto].
+    autorewrite with sep in H; sep_normal_in H.
+    assert (Heq : (Gl aloc +o (Zn (gi i j)) ===l Gl "arr" +o gid) s (emp_ph loc)).
+    { sep_split_in H; unfold_conn; simpl; f_equal; unfold_pures; clear H; nia. }
+    sep_rewrite_in mps_eq1 H; [|exact Heq]; clear Heq.
+    assert (Heq : (Sh sloc +o (Zn (nf i + 1)) ===l Sh "smem" +o ("tid" +C 1%Z)) s (emp_ph loc)).
+    { sep_split_in H; unfold_conn; simpl; f_equal; unfold_pures; clear H; nia. }
+    sep_lift_in H 9.
+    sep_rewrite_in mps_eq1 H; [|exact Heq]; clear Heq.
+    apply H.
+  } Unfocus.
+  eapply rule_seq; [hoare_forward; eauto|].
+  eapply rule_seq; [hoare_forward; eauto|].
+  eapply rule_seq.
+  hoare_forward; eauto using rule_skip.
+  { hoare_forward; eauto.
+    { eapply Hbackward.
+      Focus 2. {
+        intros s h H; sep_split_in H.
+        change_in H.
+        { unfold_pures; destruct Nat.eq_dec; try omega.
+          assert (Heq : (Sh sloc ===l Sh "smem" +o 0%Z) s (emp_ph loc)).
+          { sep_split_in H; unfold_conn; simpl; f_equal; unfold_pures; clear H; nia. }
+          sep_lift_in H 5.
+          sep_rewrite_in mps_eq1 H; [|exact Heq]; clear Heq.
+          apply H. }
+        sep_combine_in H; apply H. } Unfocus.
+      hoare_forward; eauto. }
+    { eapply Hbackward.
+      Focus 2. {
+        intros s h H; sep_split_in H.
+        change_in H.
+        { unfold_pures; destruct Nat.eq_dec; try omega.
+          assert (Heq : (Sh sloc ===l Sh "smem" +o 0%Z) s (emp_ph loc)).
+          { sep_split_in H; unfold_conn; simpl; f_equal; unfold_pures; clear H; nia. }
+          sep_lift_in H 5.
+          sep_rewrite_in mps_eq1 H; [|exact Heq]; clear Heq.
+          sep_rewrite_in (@is_array_unfold (Gl aloc) (gi i j - 1)) H; [|eauto; clear H; nia].
+          sep_normal_in H.
+          assert (Heq : (Gl aloc +o (Zn (gi i j - 1 + 0)) ===l Gl "arr" +o (gid -C 1%Z) ) s (emp_ph loc)).
+          { sep_split_in H; unfold_conn; simpl; f_equal; unfold_pures; clear H; nia. }
+          sep_lift_in H 4.
+          sep_rewrite_in mps_eq1 H; [|exact Heq]; clear Heq.
+          assert (Heq : ("t0" === f (gi i j)) s (emp_ph loc)).
+          { unfold_pures; unfold_conn; eauto. }
+          sep_lift_in H 2.
+          sep_rewrite_in mps_eq2 H; [|exact Heq].
+          apply H. }
+        clear HP1.
+        sep_combine_in H; apply H. } Unfocus. 
+      eapply rule_seq; [hoare_forward; eauto|].
+      hoare_forward; eauto. } }
+  eapply Hbackward.
+  Focus 2. {
+    instantiate (1 :=
+     !("tid" === Zn (nf i)) **
+     !("bid" === Zn (nf j)) **
+     !("arr" === aloc) **
+     !("out" === oloc) **
+     !("smem" === sloc ) **
+     is_array_p (Gl aloc) nt_gr f 0 (perm_n nt_gr) **
+     (Gl oloc +o Zn (nf i + nf j * ntrd) -->p (1, f_out (nf i + nf j * ntrd))) **
+     (Sh "smem" +o ("tid" +C 1%Z) -->p (1, f' (gi i j + 1))) **
+     (if Nat.eq_dec (nf i) 0 then Sh "smem" -->p (1, f' (nf j * ntrd)) else emp) **
+     (if Nat.eq_dec (nf i) (ntrd - 1) then Sh sloc +o Zn (ntrd + 1) -->p (1, f_sm (ntrd + 1)) else emp)).
+    intros s h H; sep_rewrite (@is_array_unfold (Gl aloc) (gi i j)); [|eauto].
+    sep_normal; sep_cancel.
+    destruct H as [[H | H] | H]; sep_split_in H; sep_split; eauto; sep_cancel.
+    { unfold_pures.
+      destruct (Nat.eq_dec (nf i) 0);  [|clear H H0; nia].
+      assert (Heq : (Gl aloc +o (Zn (gi i j + 0)) ===l Gl "arr" +o gid) s (emp_ph loc)).
+      { sep_split_in H; unfold_conn; simpl; f_equal; unfold_pures; clear H H0; nia. }
+      sep_rewrite mps_eq1; [|exact Heq]; clear Heq.
+      rewrite <-plus_n_O.
+      repeat sep_cancel.
+      unfold f'; lazymatch goal with [|- context [if ?X then _ else _]] => destruct X end; try nia.
+      lazymatch goal with [|- context [if ?X then _ else _]] => destruct X end; try nia.
+      assert (Heq : ("t0" === f (gi i j)) s (emp_ph loc)).
+      { unfold_pures; unfold_conn; eauto. }
+      rewrite Nat.add_sub.
+      sep_lift_in H3 1.
+      sep_rewrite_in mps_eq2 H3; [|exact Heq].
+      repeat sep_cancel. }
+    { unfold_pures.
+      destruct (Nat.eq_dec (nf i) 0); [|clear H H0; nia].
+      assert (Heq : (Gl aloc +o (Zn (gi i j + 0)) ===l Gl "arr" +o gid) s (emp_ph loc)).
+      { sep_split_in H; unfold_conn; simpl; f_equal; unfold_pures; clear H H0; nia. }
+      sep_rewrite mps_eq1; [|exact Heq]; clear Heq.
+      rewrite <-plus_n_O.
+      repeat sep_cancel.
+      sep_rewrite (@is_array_unfold (Gl aloc) (gi i j - 1)); [|eauto; clear H H0 H1 H2; nia].
+      sep_normal.
+      assert (Heq : (Gl aloc +o (Zn (gi i j - 1 + 0)) ===l Gl "arr" +o ("tid" +C "bid" *C Zn ntrd -C 1%Z)) s (emp_ph loc)).
+      { sep_split_in H; unfold_conn; simpl; f_equal; unfold_pures; clear H H0 H1 H2; nia. }
+      sep_rewrite mps_eq1; [|exact Heq]; clear Heq.
+      repeat sep_cancel.
+      unfold f'; lazymatch goal with [|- context [if ?X then _ else _]] => destruct X end;
+        [clear H H0 H1 H2 H3 H4 H5; nia|].
+      lazymatch goal with [|- context [if ?X then _ else _]] => destruct X end;
+        [clear H H0 H1 H2 H3 H4 H5; nia|].
+      rewrite Nat.add_sub.
+      assert (Heq : ("t0" === f (gi i j - 1 + 0)) s (emp_ph loc)).
+      { unfold_pures; unfold_conn; eauto. }
+      sep_rewrite_in mps_eq2 H5; [|exact Heq].
+      cutrewrite (nf j * ntrd - 1 = gi i j - 1 + 0); [|clear H H0 H1 H2 H3 H4 H5; nia].
+      repeat sep_cancel. }
+    { unfold_pures.
+      destruct (Nat.eq_dec (nf i) 0); [clear H H0; nia|].
+      sep_rewrite emp_unit_l; sep_rewrite_in emp_unit_l H0.
+      assert (Heq : (Gl aloc +o (Zn (gi i j + 0)) ===l Gl "arr" +o gid) s (emp_ph loc)).
+      { sep_split_in H; unfold_conn; simpl; f_equal; unfold_pures; clear H H0; nia. }
+      sep_rewrite mps_eq1; [|exact Heq]; clear Heq.
+      rewrite <-plus_n_O.
+      repeat sep_cancel.
+      assert (Heq : ("t0" === f (gi i j)) s (emp_ph loc)).
+      { unfold_pures; unfold_conn; eauto. }
+      sep_rewrite_in mps_eq2 H3; [|exact Heq].
+      unfold f'; lazymatch goal with [|- context [if ?X then _ else _]] => destruct X end;
+        [clear H H0 H1 H2 H3; nia|].
+      rewrite Nat.add_sub.
+      sep_cancel. } } Unfocus.
+  eapply rule_seq.
+  hoare_forward; eauto using rule_skip.
+  { eapply Hbackward.
+    Focus 2. {
+        intros s h H; sep_split_in H.
+        change_in H.
+        { unfold_pures; destruct (Nat.eq_dec _ (ntrd - 1)); [|clear H; false; nia].
+          assert (Heq : (Sh sloc +o Zn (ntrd + 1) ===l Sh "smem" +o (Zn ntrd +C 1%Z)) s (emp_ph loc)).
+          { sep_split_in H; unfold_conn; simpl; f_equal; unfold_pures; clear H; nia. }
+          sep_lift_in H 5.
+          sep_rewrite_in mps_eq1 H; [|exact Heq]; clear Heq.
+          apply H. }
+        sep_combine_in H; apply H. } Unfocus.
+    hoare_forward; eauto.
+    hoare_forward; eauto.
+    { eapply Hbackward.
+      Focus 2. {
+        intros s h H; sep_split_in H.
+        change_in H.
+        { unfold_pures.
+          sep_rewrite_in (@is_array_unfold (Gl aloc) (gi i j + 1)) H; [|eauto; clear H; nia].
+          sep_normal_in H.
+          assert (Heq : (Gl aloc +o (Zn (gi i j + 1 + 0)) ===l Gl "arr" +o (gid +C 1%Z) ) s (emp_ph loc)).
+          { sep_split_in H; unfold_conn; simpl; f_equal; unfold_pures; clear H; nia. }
+          sep_lift_in H 2.
+          sep_rewrite_in mps_eq1 H; [|exact Heq]; clear Heq.
+          apply H. }
+        sep_combine_in H; apply H. } Unfocus. 
+      eapply rule_seq; [hoare_forward; eauto|].
+      hoare_forward; eauto. } }
+
+  eapply Hbackward.
+  Focus 2. {
+    instantiate (1 :=
+     !("tid" === Zn (nf i)) **
+     !("bid" === Zn (nf j)) **
+     !("arr" === aloc) **
+     !("out" === oloc) **
+     !("smem" === sloc ) **
+     is_array_p (Gl aloc) nt_gr f 0 (perm_n nt_gr) **
+     (Gl oloc +o Zn (nf i + nf j * ntrd) -->p (1, f_out (nf i + nf j * ntrd))) **
+     (Sh "smem" +o ("tid" +C 1%Z) -->p (1, f' (gi i j + 1))) **
+     (if Nat.eq_dec (nf i) 0 then Sh "smem" -->p (1, f' (nf j * ntrd)) else emp) **
+     (if Nat.eq_dec (nf i) (ntrd - 1) then Sh "smem" +o Zn (ntrd + 1) -->p (1, f' ((nf j + 1) * ntrd + 1)) else emp)).
+    intros s h H; sep_normal.
+    destruct H as [[H | H] | H]; sep_split_in H; sep_split; eauto; repeat sep_cancel.
+    { unfold_pures.
+      destruct (Nat.eq_dec _ (ntrd - 1)); [|clear H H0 H1 H2; false; nia].
+      assert (Heq : (Sh "smem" +o (Zn ntrd +C 1%Z) ===l Sh "smem" +o Zn (ntrd + 1)) s (emp_ph loc)).
+      { sep_split_in H; unfold_conn; simpl; f_equal; unfold_pures; clear H H0 H1 H2 H3; nia. }
+      sep_rewrite_in mps_eq1 H3; [|exact Heq]; clear Heq.
+      unfold f'; lazymatch goal with [|- context [if ?X then _ else _]] => destruct X end; try (false; nia).
+      apply H3. }
+    { unfold_pures.
+      sep_rewrite (@is_array_unfold (Gl aloc) (gi i j + 1)); [|eauto; clear H H0 H1 H2; nia].
+      sep_normal.
+      assert (Heq : (Gl aloc +o (Zn (gi i j + 1 + 0)) ===l Gl "arr" +o (gid +C 1%Z) ) s (emp_ph loc)).
+      { sep_split_in H; unfold_conn; simpl; f_equal; unfold_pures; clear H; nia. }
+      sep_lift 1.
+      sep_rewrite mps_eq1; [|exact Heq]; clear Heq.
+      repeat sep_cancel.
+      destruct (Nat.eq_dec _ (ntrd - 1)); [|clear H0 H1 H2 H3 H4 H5; nia].
+      unfold f'; lazymatch goal with [|- context [if ?X then _ else _]] => destruct X end; try (false; nia).
+      rewrite Nat.add_sub.
+      assert (Heq : ("t0" === f ((nf j + 1) * ntrd)) s (emp_ph loc)).
+      { unfold_pures; unfold_conn; simpl; rewrite HP; f_equal; nia. }
+      sep_rewrite_in mps_eq2 H5; [|exact Heq]; clear Heq.
+      assert (Heq : (Sh "smem" +o (Zn ntrd +C 1%Z) ===l Sh "smem" +o Zn (ntrd + 1)) s (emp_ph loc)).
+      { sep_split_in H; unfold_conn; simpl; f_equal; unfold_pures; clear H H0 H1 H2 H3 H4 H5; nia. }
+      sep_rewrite_in mps_eq1 H5; [|exact Heq]; clear Heq.
+      apply H5. }
+    { unfold_pures.
+      destruct (Nat.eq_dec _ (ntrd - 1)); [clear H H0 H1 H2 H3; nia|]; eauto.  } } Unfocus.
+  eapply rule_seq.
+  (* The following tactics cannot be replaced with hoare_forward
+  because of a buggy behavior of tauto used by hoare_forward. tauto
+  removes useless hypothesis for proving the goal, and when the goal
+  contains some unification variables, it can't look removed
+  hypothesis. *)
+  idtac "called"; eapply Hforward;
+         [ eapply Hbackward;
+            [ eapply rule_frame; [ apply rule_barrier | split; simpl in *; destruct H]
+            | autounfold ; simpl; repeat rewrite MyVector.init_spec in * ]
+         | idtac ]; eauto.
+  { intros s h H.
+
+    sep_split_in H.
+    sep_normal.
+    change_in H.    
+    { unfold_pures.
+      assert (Heq : (Sh "smem" +o ("tid" +C 1%Z) ===l Sh sloc +o (Zn (nf i + 1)) ) s (emp_ph loc)).
+      { unfold_conn; simpl; f_equal; clear H; unfold lt; nia. }
+      sep_lift_in H 2.
+      sep_rewrite_in mps_eq1 H; [|apply Heq]; clear Heq.
+      assert (Heq : s ||= (if Nat.eq_dec (nf i) 0 then Sh "smem" -->p (1,  f' (nf j * ntrd)) else emp) <=>
+                          (if Nat.eq_dec (nf i) 0 then Sh sloc -->p (1,  f' (nf j * ntrd)) else emp)).
+      { destruct (Nat.eq_dec _ 0); try reflexivity.
+        apply mps_eq1; unfold_conn; simpl; f_equal; nia. }
+      sep_rewrite_in Heq H; clear Heq.
+      assert (Heq : s ||=
+        (if Nat.eq_dec (nf i) (ntrd - 1) then Sh "smem" +o Zn (ntrd + 1) -->p (1,  f' ((nf j + 1) * ntrd + 1)) else emp)
+        <=>
+        (if Nat.eq_dec (nf i) (ntrd - 1) then Sh sloc +o Zn (ntrd + 1) -->p (1,  f' ((nf j + 1) * ntrd + 1)) else emp)).
+      { destruct (Nat.eq_dec _ (ntrd - 1)); try reflexivity.
+        apply mps_eq1; unfold_conn; simpl; f_equal; nia. }
+      sep_rewrite_in Heq H; clear Heq.
+      apply H. }
+    sep_normal_in H0; do 2 sep_cancel.
+    sep_combine_in H1; apply H1. }
+  unfold BS at 2, BS0; simpl; rewrite MyVector.init_spec.
+  eapply Hbackward.
+  Focus 2. { 
+    intros s h H.
+    sep_split_in H.
+    sep_rewrite_in (@is_array_unfold (Sh sloc) (nf i)) H; [|destruct (Fin.to_nat i); clear H; simpl; omega].
+    sep_normal_in H.
+    sep_lift_in H 2; sep_rewrite_in (@is_array_unfold (Sh sloc) 0) H; [|destruct (Fin.to_nat i); clear H; simpl; omega].
+    sep_normal_in H.
+    sep_lift_in H 2; sep_rewrite_in (@is_array_unfold (Sh sloc) 0) H; [|destruct (Fin.to_nat i); clear H; simpl; omega].
+    sep_normal_in H.
+    change_in H.
+    { unfold_pures.
+      assert (Heq : (Sh sloc +o Zn (0 + S (0 + S (nf i + 0))) ===l Sh sloc +o ("tid" +C 2%Z)) s (emp_ph loc)).
+      { rewrite !plus_O_n, <-plus_n_O, !Nat2Z.inj_succ, <-!Z.add_1_r.
+        unfold_conn; simpl; f_equal; clear H; unfold lt; omega. }
+      sep_rewrite_in mps_eq1 H; [|exact Heq]; clear Heq.
+      assert (Heq : (Sh sloc +o Zn (0 + S (nf i + 0)) ===l Sh sloc +o ("tid" +C 1%Z)) s (emp_ph loc)).
+      { rewrite !plus_O_n, <-plus_n_O, !Nat2Z.inj_succ, <-!Z.add_1_r.
+        unfold_conn; simpl; f_equal; clear H; unfold lt; omega. }
+      sep_lift_in H 4; sep_rewrite_in mps_eq1 H; [|exact Heq]; clear Heq.
+      assert (Heq : (Sh sloc +o Zn (nf i + 0) ===l Sh sloc +o "tid") s (emp_ph loc)).
+      { unfold_conn; simpl; f_equal; clear H; unfold lt in *; nia. }
+      sep_lift_in H 6; sep_rewrite_in mps_eq1 H; [|exact Heq]; clear Heq.
+      assert (Heq : (Gl oloc +o Zn (gi i j) ===l Gl oloc +o gid) s (emp_ph loc)).
+      { unfold_conn; simpl; f_equal; clear H; unfold lt in *; nia. }
+      sep_lift_in H 8; sep_rewrite_in mps_eq1 H; [|exact Heq]; clear Heq.
+      apply H. } 
+    sep_combine_in H; apply H. } Unfocus.
+  repeat (eapply rule_seq; [hoare_forward; eauto|]).
+  eapply Hforward; [hoare_forward; eauto|].
+  intros s h H.
+  sep_split_in H; sep_cancel.
+  unfold_pures.
+  sep_rewrite (@is_array_unfold (Sh sloc) (nf i)); [|destruct (Fin.to_nat i); clear H; simpl; omega].
+  sep_normal.
+  sep_lift 3; sep_rewrite (@is_array_unfold (Sh sloc) 0); [|destruct (Fin.to_nat i); clear H; simpl; omega].
+  sep_normal.
+  sep_lift 2. sep_rewrite (@is_array_unfold (Sh sloc) 0). 2: destruct (Fin.to_nat i). 2: clear H H0. 2: simpl.
+  2: generalize dependent x. 2: clear. 2: intros. 2: omega.
+  sep_normal_in H0. clear H. sep_normal.
+  assert (Heq : (Sh sloc +o Zn (0 + S (0 + S (nf i + 0))) ===l Sh "smem" +o ("tid" +C 2%Z)) s (emp_ph loc)).
+  { rewrite !plus_O_n, <-plus_n_O, !Nat2Z.inj_succ, <-!Z.add_1_r.
+    unfold_conn; simpl; f_equal; unfold lt; omega. }
+  sep_rewrite mps_eq1; [|exact Heq]; clear Heq.
+  assert (Heq : (Sh sloc +o Zn (0 + S (nf i + 0)) ===l Sh "smem" +o ("tid" +C 1%Z)) s (emp_ph loc)).
+  { rewrite !plus_O_n, <-plus_n_O, !Nat2Z.inj_succ, <-!Z.add_1_r.
+    unfold_conn; simpl; f_equal; unfold lt; omega. }
+  sep_lift 4; sep_rewrite mps_eq1; [|exact Heq]; clear Heq.
+  assert (Heq : (Sh sloc +o Zn (nf i + 0) ===l Sh "smem" +o "tid") s (emp_ph loc)).
+  { unfold_conn; simpl; f_equal; clear H0; unfold lt in *. nia. }
+  sep_lift 7; sep_rewrite mps_eq1; [|exact Heq]; clear Heq.
+  assert (Heq : (Gl oloc +o Zn (gi i j) ===l Gl "out" +o gid) s (emp_ph loc)).
+  { unfold_conn; simpl; f_equal; clear H0; unfold lt in *; nia. }
+  sep_lift 6; sep_rewrite mps_eq1; [|exact Heq]; clear Heq.
+  assert (Heq : ((f' (gi i j) + f' (gi i j + 1))%Z +C f' (gi i j + 2) ===
+                 "t0" +C "t1" +C "t2") s (emp_ph loc)).
+  { unfold_conn; simpl.
+    do 2 f_equal; try rewrite HP; try rewrite HP0; try rewrite HP1; f_equal; try omega. }
+  sep_rewrite mps_eq2; [|exact Heq]; clear Heq.
+  repeat sep_cancel.
+Qed.
+Section Stencil_seq.
